.

pure/Data.v
@@ -4,29 +4,295 @@ Require Import Coq.Classes.RelationClasses.
 Require Import Coq.Lists.List.
 Require Import Coq.micromega.Lia.
 Require Import Coq.Program.Basics.
-Require Import DschingisKhan.pure.FunFacts.
 Require Import DschingisKhan.pure.MyStructures.
 Require Import DschingisKhan.pure.MyUtilities.
 
-Module BinaryTrees.
+Module LinkedLists.
 
   Import ListNotations EqFacts MyUtilities BasicSetoidTheory BasicPosetTheory.
 
+  Section LIST_EXTENSIONALITY.
+
+  Definition good_idx_implies_nth_error_ne_None {A : Type} (xs : list A) :
+    forall idx : nat,
+    idx < length xs ->
+    nth_error xs idx <> None.
+  Proof.
+    induction xs as [ | x xs IH].
+    - intros idx H_lt.
+      exact (lt_elim_n_lt_0 idx H_lt).
+    - intros [ | idx'] H_lt.
+      + exact (Some_ne_None x).
+      + simpl in *.
+        apply IH.
+        exact (lt_elim_S_n_lt_S_m idx' (length xs) H_lt).
+  Defined.
+
+  Definition listEXT_view {A : Type} (xs : list A) : forall idx : nat, {ret : option A | idx < length xs -> ret <> None} :=
+    fun idx : nat =>
+    exist _ (nth_error xs idx) (good_idx_implies_nth_error_ne_None xs idx)
+  .
+
+  Definition listExt_view {A : Type} (xs : list A) : nat -> option A :=
+    fun idx : nat =>
+    proj1_sig (listEXT_view xs idx)
+  .
+
+  Lemma list_extensionality {A : Type} :
+    forall xs1 : list A,
+    forall xs2 : list A,
+    xs1 = xs2 <-> (forall n : nat, listExt_view xs1 n = listExt_view xs2 n).
+  Proof with discriminate || eauto.
+    cbn.
+    induction xs1 as [ | x1 xs1 IH]; intros [ | x2 xs2]; simpl; split...
+    - intros H_false.
+      contradiction (Some_ne_None x2).
+      symmetry; exact (H_false 0).
+    - intros H_false.
+      contradiction (Some_ne_None x1).
+      exact (H_false 0).
+    - intros H_eq.
+      rewrite H_eq.
+      reflexivity.
+    - intros H_eq.
+      assert (claim1 := H_eq 0).
+      simpl in claim1; apply Some_inj in claim1; subst x2.
+      apply eq_congruence, IH.
+      exact (fun n => H_eq (S n)).
+  Qed.
+
+  Lemma listExt_map {A : Type} {B : Type} (f : A -> B) (xs : list A) :
+    (forall n : nat, listExt_view (map f xs) n = (fmapMaybe f) (listExt_view xs n)).
+  Proof with discriminate || eauto.
+    cbn.
+    induction xs as [ | x xs IH]; simpl.
+    - intros [ | n']...
+    - intros [ | n']; simpl...
+  Qed.
+
+  Definition safeLookat {A : Type} (xs : list A) : forall idx : nat, idx < length xs -> A :=
+    fun idx : nat =>
+    match listEXT_view xs idx with
+    | exist _ xr H_xr => fun H_idx : idx < length xs => fromJust xr (H_xr H_idx)
+    end
+  .
+
+  Lemma listExt_safeLookat {A : Type} (xs : list A) :
+    forall n : nat,
+    listExt_view xs n =
+    match n_le_m_or_m_lt_n_holds_for_any_n_and_any_m (length xs) n with
+    | left H_le => None
+    | right H_lt => Some (safeLookat xs n H_lt)
+    end.
+  Proof with eauto.
+    intros n; cbn.
+    destruct (n_le_m_or_m_lt_n_holds_for_any_n_and_any_m (length xs)) as [H_le | H_lt].
+    - apply nth_error_None...
+    - apply (proj2 (fromJust_spec (nth_error xs n) (fromJust (nth_error xs n) (good_idx_implies_nth_error_ne_None xs n H_lt))))...
+  Qed.
+
+  End LIST_EXTENSIONALITY.
+
+  Section LIST_SWAP.
+
+  Context {A : Type}.
+
+  Definition addIndices_aux : list A -> nat -> list (A * nat) :=
+    fold_right (fun x : A => fun acc : nat -> list (A * nat) => fun n : nat => (x, n) :: acc (1 + n)) (fun n : nat => [])
+  .
+
+  Lemma addIndices_aux_unfold :
+    forall xs : list A,
+    forall n : nat,
+    addIndices_aux xs n =
+    match xs with
+    | [] => []
+    | hd_xs :: tl_xs => (hd_xs, n) :: addIndices_aux tl_xs (S n)
+    end.
+  Proof with eauto.
+    induction xs as [ | x xs IH]; simpl...
+  Qed.
+
+  Definition addIndices (xs : list A) : list (A * nat) :=
+    addIndices_aux xs 0
+  .
+
+  Lemma addIndices_unfold :
+    forall xs : list A,
+    addIndices xs =
+    match xs with
+    | [] => []
+    | hd_xs :: tl_xs => (hd_xs, 0) :: map (fun it => (fst it, 1 + snd it)) (addIndices tl_xs)
+    end.
+  Proof with eauto.
+    unfold addIndices; cbn.
+    intros xs1; generalize 0 as n; intros n.
+    rewrite addIndices_aux_unfold at 1.
+    destruct xs1 as [ | x1 xs1]...
+    apply eq_congruence.
+    clear x1; revert n; induction xs1 as [ | x1 xs1 IH]; simpl...
+    intros n; apply eq_congruence; exact (IH (S n)).
+  Qed.
+
+  Lemma addIndices_length :
+    forall xs : list A,
+    length (addIndices xs) = length xs.
+  Proof with eauto.
+    induction xs as [ | x xs IH]...
+    rewrite addIndices_unfold; simpl...
+    apply eq_congruence; rewrite map_length...
+  Qed.
+
+  Lemma addIndices_map_fst :
+    forall xs : list A,
+    map fst (addIndices xs) = xs.
+  Proof with eauto.
+    induction xs as [ | x xs IH]...
+    rewrite addIndices_unfold; simpl.
+    apply eq_congruence.
+    rewrite <- IH at 2.
+    generalize (addIndices xs) as its.
+    clear x xs IH.
+    induction its; simpl...
+    apply eq_congruence...
+  Qed.
+
+  Lemma addIndices_map_snd :
+    forall xs : list A,
+    forall idx : nat,
+    idx < length xs <-> nth_error (map snd (addIndices xs)) idx = Some idx.
+  Proof with eauto.
+    intros xs idx; split.
+    { unfold addIndices; replace idx with (0 + idx) at 3...
+      generalize 0 as n; revert idx; induction xs as [ | x xs IH]; simpl; intros i n H_lt.
+      - exact (lt_elim_n_lt_0 i H_lt).
+      - destruct i as [ | i']; simpl.
+        + apply eq_congruence; lia.
+        + apply lt_elim_S_n_lt_S_m in H_lt.
+          rewrite (IH i' (S n) H_lt).
+          apply eq_congruence; lia.
+    }
+    { intros H_Some.
+      rewrite <- addIndices_length, <- (map_length snd).
+      apply nth_error_Some.
+      rewrite H_Some.
+      discriminate.
+    }
+  Qed.
+
+  Lemma listExt_addIndices (xs : list A) :
+    forall idx : nat,
+    match listExt_view (addIndices xs) idx with
+    | None => idx >= length xs
+    | Some (x, n) => listExt_view xs idx = Some x /\ idx = n
+    end.
+  Proof with discriminate || eauto.
+    intros idx; cbn.
+    destruct (nth_error (addIndices xs) idx) as [[x n] | ] eqn: H_obs_addIndices.
+    - assert (H_nth : nth idx (addIndices xs) (x, n) = (x, n)) by now apply nth_error_nth.
+      assert (claim1 := (map_nth fst (addIndices xs) (x, n) idx)).
+      assert (claim2 := (map_nth snd (addIndices xs) (x, n) idx)).
+      rewrite H_nth in claim1, claim2; cbn in claim1, claim2.
+      rewrite addIndices_map_fst in claim1.
+      assert (H_length : idx < length xs).
+      { rewrite <- addIndices_length. apply nth_error_Some. rewrite H_obs_addIndices... }
+      assert (H_n_eq_idx := proj1 (addIndices_map_snd xs idx) H_length).
+      apply nth_error_nth with (d := n) in H_n_eq_idx.
+      rewrite claim2 in H_n_eq_idx.
+      split... rewrite <- claim1; apply nth_error_nth'...
+    - rewrite <- addIndices_length; apply nth_error_None...
+  Qed.
+
+  Definition listSwap_aux (xs : list A) (idx1 : nat) (idx2 : nat) (default_val : A) (idx : nat) : A :=
+    let x1 : A := maybe default_val id (nth_error xs idx1) in
+    let x2 : A := maybe default_val id (nth_error xs idx2) in
+    if eq_dec_nat idx idx1 then x2 else
+    if eq_dec_nat idx idx2 then x1 else
+    default_val
+  .
+
+  Definition listSwap (idx1 : nat) (idx2 : nat) : list A -> list A :=
+    fun xs : list A =>
+    map (uncurry (listSwap_aux xs idx1 idx2)) (addIndices xs)
+  .
+
+  Lemma listSwap_length :
+    forall idx1 : nat,
+    forall idx2 : nat,
+    forall xs : list A,
+    length (listSwap idx1 idx2 xs) = length xs.
+  Proof.
+    unfold listSwap; intros idx1 idx2 xs.
+    transitivity (length (addIndices xs)); [apply map_length | apply addIndices_length].
+  Qed.
+
+  Lemma listExt_swap :
+    forall idx1 : nat,
+    forall idx2 : nat,
+    forall xs : list A,
+    forall idx : nat,
+    listExt_view (listSwap idx1 idx2 xs) idx =
+    fmapMaybe (uncurry (listSwap_aux xs idx1 idx2)) (listExt_view (addIndices xs) idx).
+  Proof.
+    intros idx1 idx2 xs idx.
+    exact (listExt_map (uncurry (listSwap_aux xs idx1 idx2)) (addIndices xs) idx).
+  Qed.
+
+  Theorem listSwap_main_spec :
+    forall xs : list A,
+    forall idx1 : nat,
+    forall val1 : A,
+    listExt_view xs idx1 = Some val1 ->
+    forall idx2 : nat,
+    forall val2 : A,
+    listExt_view xs idx2 = Some val2 ->
+    forall idx : nat,
+    forall val : A,
+    listExt_view xs idx = Some val ->
+    match listExt_view (listSwap idx1 idx2 xs) idx with
+    | None => False
+    | Some x => x =
+      if eq_dec_nat idx idx1 then val2 else
+      if eq_dec_nat idx idx2 then val1 else
+      val
+    end.
+  Proof with discriminate || eauto.
+    cbn; intros xs idx1 val1 H_idx1 idx2 val2 H_idx2 idx val H_idx.
+    assert (claim1 := listExt_swap idx1 idx2 xs idx).
+    assert (claim2 := listExt_addIndices xs idx).
+    cbn in claim1, claim2; rewrite claim1.
+    unfold fmapMaybe, listExt_view, listSwap_aux; simpl.
+    destruct (nth_error (addIndices xs) idx) as [[x n] |] eqn: H_obs_addIndices; simpl in *.
+    - destruct claim2 as [H_obs_xs H_obs_idx]; subst n.
+      destruct (eq_dec_nat idx idx1) as [H_yes1 | H_no1].
+      { subst idx. rewrite H_idx2... }
+      destruct (eq_dec_nat idx idx2) as [H_yes2 | H_no2].
+      { subst idx. rewrite H_idx1... }
+      congruence.
+    - apply nth_error_None in claim2; rewrite claim2 in H_idx...
+  Qed.
+
+  End LIST_SWAP.
+
+End LinkedLists.
+
+Module BinaryTrees.
+
+(*Import ListNotations EqFacts MyUtilities BasicSetoidTheory BasicPosetTheory LinkedLists.
+
+  Local Open Scope program_scope.
+
   Section INDICES_OF_BINARY_TREES.
 
-  Inductive dir_t : Set :=
-  | Dir_left : dir_t
-  | Dir_right : dir_t
-  .
+  Inductive dir_t : Set := Dir_left : dir_t | Dir_right : dir_t.
 
-  Definition encode : list dir_t -> nat :=
-    fun idx : list dir_t =>
-    fold_left (fun code : nat => @dir_t_rec (fun _ : dir_t => nat) (2 * code + 1) (2 * code + 2)) idx 0
-  .
+  Definition index_t : Set := list dir_t.
+
+  Definition encode (idx : index_t) := fold_left (fun code : nat => @dir_t_rec (fun _ : dir_t => nat) (2 * code + 1) (2 * code + 2)) idx 0.
 
   Lemma encode_inj :
-    forall idx1 : list dir_t,
-    forall idx2 : list dir_t,
+    forall idx1 : index_t,
+    forall idx2 : index_t,
     encode idx1 = encode idx2 ->
     idx1 = idx2.
   Proof with lia || eauto.
@@ -44,7 +310,7 @@ Module BinaryTrees.
 
   Lemma decodable :
     forall code : nat,
-    {idx : list dir_t | encode idx = code}.
+    {idx : index_t | encode idx = code}.
   Proof with lia || eauto.
     induction code as [[ | code'] IH] using Wf_nat.lt_wf_rec.
     - exists ([])...
@@ -67,10 +333,7 @@ Module BinaryTrees.
       + pose (Nat.mod_bound_pos code 2)...
   Defined.
 
-  Definition decode : nat -> list dir_t :=
-    fun code : nat =>
-    proj1_sig (decodable code)
-  .
+  Definition decode code : index_t := proj1_sig (decodable code).
 
 (* (* Example "decode" *)
   Compute (decode 14).
@@ -91,11 +354,26 @@ Module BinaryTrees.
   Global Opaque decode.
 
   Lemma decode_encode :
-    forall idx : list dir_t,
+    forall idx : index_t,
     decode (encode idx) = idx.
   Proof.
     intro idx. apply encode_inj.
     now rewrite encode_decode with (code := encode idx).
+  Qed.
+
+  Global Program Instance index_t_isPoset : isPoset index_t :=
+    { Poset_requiresSetoid :=
+      {| eqProp := @eq index_t; Setoid_requiresEquivalence := @eq_equivalence index_t |}
+    ; leProp := fun idx1 idx2 => encode idx1 <= encode idx2
+    }
+  .
+  Next Obligation with eauto with *.
+    split...
+  Qed.
+  Next Obligation with eauto with *.
+    intros idx1 idx2; cbn. unfold flip; split.
+    - intros ?; subst...
+    - intros [H_le H_ge]. apply encode_inj...
   Qed.
 
   End INDICES_OF_BINARY_TREES.
@@ -108,240 +386,90 @@ Module BinaryTrees.
   Global Arguments BT_null {Elem}.
   Global Arguments BT_node {Elem}.
 
-  Definition option_elem {Elem : Type} : bintree Elem -> option Elem :=
-    fun t : bintree Elem =>
+  Polymorphic Definition option2list {A : Type} : option A -> list A :=
+    @option_rect A (fun _ => list A) (fun x : A => [x]) []
+  .
+
+  Polymorphic Definition pair2list {A : Type} : A * A -> list A :=
+    fun '(x1, x2) => [x1; x2]
+  .
+
+  Section BINARYTREE_BASIC_OPERATIONS.
+
+  Context {Elem : Type}.
+
+  Definition option_elem t : option Elem :=
     match t with
     | BT_null => None
     | BT_node t_l t_e t_r => Some t_e
     end
   .
 
-  Definition option_children_pair {Elem : Type} : bintree Elem -> option (bintree Elem * bintree Elem) :=
-    fun t : bintree Elem =>
+  Definition option_children_pair t : option (bintree Elem * bintree Elem) :=
     match t with
     | BT_null => None
     | BT_node t_l t_e t_r => Some (t_l, t_r)
     end
   .
 
-  Section BINARY_TREE_ACCESSORIES.
+  Definition option_subtree_init t : option (bintree Elem) := Some t.
 
-  Polymorphic Definition option2list {A : Type} : option A -> list A :=
-    @option_rect A (fun _ => list A) (fun x : A => [x]) []
-  .
-
-  Polymorphic Definition pair2list {A : Type} : A * A -> list A :=
-    fun pr : A * A =>
-    [fst pr; snd pr]
-  .
-
-  Context {Elem : Type}.
-
-  Definition option_subtree_init : ((bintree Elem) -> option (bintree Elem)) :=
-    fun t => Some t
-  .
-
-  Definition option_subtree_step : dir_t -> ((bintree Elem) -> option (bintree Elem)) -> ((bintree Elem) -> option (bintree Elem)) :=
-    fun d acc t =>
+  Definition option_subtree_step d acc t : option (bintree Elem) :=
     match t with
     | BT_null => None
     | BT_node t_l t_e t_r => acc (@dir_t_rect (fun _ => bintree Elem) t_l t_r d)
     end
   .
 
-  Definition option_subtree : list dir_t -> (bintree Elem -> option (bintree Elem)) :=
-    fold_right option_subtree_step option_subtree_init
-  .
-
-  Lemma option_subtree_unfold idx t :
-    option_subtree idx t =
+  Definition option_subtree : index_t -> bintree Elem -> option (bintree Elem) :=
+    fix option_subtree_fix (idx : list dir_t) (t : bintree Elem) {struct idx} : option (bintree Elem) :=
     match idx with
     | [] => Some t
     | d :: idx =>
       match t with
       | BT_null => None
-      | BT_node t_l t_e t_r => option_subtree idx (@dir_t_rect (fun _ => bintree Elem) t_l t_r d)
+      | BT_node t_l t_e t_r => option_subtree_fix idx (@dir_t_rect (fun _ : dir_t => bintree Elem) t_l t_r d)
       end
-    end.
-  Proof. induction idx; eauto. Qed.
+    end
+  .
 
-  Inductive occurs (t : bintree Elem) : list dir_t -> bintree Elem -> Prop :=
-  | Occurs_0 :
-    occurs t [] t
-  | Occurs_l :
-    forall idx : list dir_t,
-    forall l : bintree Elem,
-    forall e : Elem,
-    forall r : bintree Elem,
-    occurs t idx l ->
-    occurs t (Dir_left :: idx) (BT_node l e r)
-  | Occurs_r :
-    forall idx : list dir_t,
-    forall l : bintree Elem,
-    forall e : Elem,
-    forall r : bintree Elem,
-    occurs t idx r ->
-    occurs t (Dir_right :: idx) (BT_node l e r)
+  Definition extract_elements := flat_map (option2list ∘ option_elem).
+
+  Definition extract_children := flat_map (@concat (bintree Elem) ∘ option2list ∘ option_map pair2list ∘ option_children_pair).
+
+  Inductive occurs t : index_t -> bintree Elem -> Prop :=
+  | Occurs_0
+    : occurs t [] t
+  | Occurs_l ds l e r
+    (H_l : occurs t ds l)
+    : occurs t (Dir_left :: ds) (BT_node l e r)
+  | Occurs_r ds l e r
+    (H_r : occurs t ds r)
+    : occurs t (Dir_right :: ds) (BT_node l e r)
   .
 
   Local Hint Constructors occurs : core.
 
-  Theorem option_subtree_occurs :
-    forall t : bintree Elem,
-    forall idx : list dir_t,
-    forall root : bintree Elem,
-    occurs t idx root <-> option_subtree idx root = Some t.
+  Lemma occurs_iff t ds root :
+    occurs t ds root <->
+    option_subtree ds root = Some t.
   Proof with discriminate || eauto.
-    unfold option_subtree. intros t idx root. split.
-    - intros X; induction X...
-    - revert t root. induction idx as [ | [ | ] idx IH]; simpl; intros t root H_eq.
-      { apply injSome in H_eq; subst root... }
-      all: destruct root as [ | l e r]...
+    split. intros X; induction X... revert t root.
+    induction ds as [ | [ | ] ds IH]; simpl; intros t root H_eq.
+    { apply injSome in H_eq; subst... }
+    all: destruct root as [ | l e r]...
   Qed.
 
-  Inductive qtrav_spec : list (bintree Elem) -> list Elem -> Prop :=
-  | qtrav_spec1
-    : qtrav_spec [] []
-  | qtrav_spec2 ts es
-    (IH_spec : qtrav_spec ts es)
-    : qtrav_spec (BT_null :: ts) es
-  | qtrav_spec3 t_l t_e t_r ts es
-    (IH_spec : qtrav_spec ((ts ++ [t_l]) ++ [t_r]) es)
-    : qtrav_spec (BT_node t_l t_e t_r :: ts) (t_e :: es)
+  Fixpoint getRank (t : bintree Elem) : nat :=
+    match t with
+    | BT_null => 0
+    | BT_node t_l t_e t_r => 1 + max (getRank t_l) (getRank t_r)
+    end
   .
 
-  Local Hint Constructors qtrav_spec : core.
+  Definition toList root : list Elem := flat_map option2list (map (fun idx => maybe None option_elem (option_subtree (decode idx) root)) (seq 0 (2 ^ getRank root - 1))).
 
-  Definition qtrav :
-    { qtrav_body : list (bintree Elem) -> list Elem
-    | forall ts : list (bintree Elem), forall xs : list Elem, qtrav_spec ts xs <-> qtrav_body ts = xs
-    }.
-  Proof with eauto.
-    set (cnt :=
-      fix cnt_fix (t : bintree Elem) {struct t} : nat :=
-      match t with
-      | BT_null => 1
-      | BT_node t_l t_e t_r => 1 + cnt_fix t_l + cnt_fix t_r
-      end
-    ).
-    set (f := fun ts => list_sum (map cnt ts)).
-    set (R := fun ts1 ts2 => f ts1 < f ts2).
-    enough (to_show : forall ts, {rslt : list Elem | forall xs, qtrav_spec ts xs <-> rslt = xs}).
-    { exists (fun ts => proj1_sig (to_show ts)). exact (fun ts => proj2_sig (to_show ts)). }
-    intros ts; pattern ts; revert ts.
-    apply FunFacts.well_founded_recursion_with_nat_lt with (get_rank := f) (LT := R)...
-    intros [ | [ | t_l t_e t_r] ts] IH.
-    - exists ([]); intros xs; split; intros H_spec.
-      + inversion H_spec; subst...
-      + subst...
-    - assert (IH_arg : R ts (BT_null :: ts)).
-      { unfold R, f. cbn; constructor. }
-      destruct (IH ts IH_arg) as [rslt H_rslt].
-      exists (rslt); intros xs; split; intros H_spec.
-      + inversion H_spec; subst. apply H_rslt...
-      + subst. constructor; apply H_rslt...
-    - assert (IH_arg : R ((ts ++ [t_l]) ++ [t_r]) (BT_node t_l t_e t_r :: ts)).
-      { unfold R, f. cbn; unfold Peano.lt.
-        do 2 rewrite map_last. do 2 rewrite list_sum_app; cbn.
-        do 2 rewrite Nat.add_0_r. rewrite <- Nat.add_assoc at 1.
-        rewrite Nat.add_comm; constructor.
-      }
-      destruct (IH ((ts ++ [t_l]) ++ [t_r]) IH_arg) as [rslt H_rslt].
-      exists (t_e :: rslt); intros xs; split; intros H_spec.
-      + inversion H_spec; subst. apply f_equal, H_rslt...
-      + subst. constructor; apply H_rslt...
-  Defined.
-
-  Lemma qtrav_unfold queue :
-    proj1_sig qtrav queue =
-    match queue with
-    | [] => []
-    | BT_null :: queue_tail => proj1_sig qtrav queue_tail
-    | BT_node t_l t_e t_r :: queue_tail => t_e :: proj1_sig qtrav ((queue_tail ++ [t_l]) ++ [t_r])
-    end.
-  Proof with eauto.
-    destruct qtrav as [qtrav_body H_qtrav_body]; simpl.
-    destruct queue as [ | [ | t_l t_e t_r] queue_tail]; simpl; apply H_qtrav_body...
-    all: constructor; apply H_qtrav_body...
-  Qed.
-
-  Definition toList_step := proj1_sig qtrav.
-
-  Lemma toList_step_unfold ts :
-    toList_step ts =
-    match ts with
-    | [] => []
-    | BT_null :: ts_tail => toList_step ts_tail
-    | BT_node t_l t_e t_r :: ts_tail => t_e :: toList_step (ts_tail ++ [t_l; t_r])
-    end.
-  Proof with eauto.
-    unfold toList_step; rewrite qtrav_unfold with (queue := ts) at 1.
-    destruct ts as [ | [ | t_l t_e t_r] ts_tail]...
-    rewrite <- app_assoc at 1; replace ([t_l] ++ [t_r]) with ([t_l; t_r])...
-  Qed.
-
-  Global Opaque toList_step.
-
-  Local Open Scope program_scope.
-
-  Definition extract_elements : list (bintree Elem) -> list Elem :=
-    flat_map (option2list ∘ option_elem)
-  .
-
-  Lemma extract_elements_unfold :
-    forall ts : list (bintree Elem),
-    extract_elements ts =
-    match ts with
-    | [] => []
-    | BT_null :: ts_tail => extract_elements ts_tail
-    | BT_node t_l t_e t_r :: ts_tail => t_e :: extract_elements ts_tail
-    end.
-  Proof.
-    destruct ts as [ | [ | ? ? ?] ?]; reflexivity.
-  Qed.
-
-  Definition extract_children : list (bintree Elem) -> list (bintree Elem) :=
-    flat_map (@concat (bintree Elem) ∘ option2list ∘ option_map pair2list ∘ option_children_pair)
-  .
-
-  Lemma extract_children_unfold :
-    forall ts : list (bintree Elem),
-    extract_children ts =
-    match ts with
-    | [] => []
-    | BT_null :: ts_tail => extract_children ts_tail
-    | BT_node t_l t_e t_r :: ts_tail => [t_l; t_r] ++ extract_children ts_tail
-    end.
-  Proof.
-    destruct ts as [ | [ | ? ? ?] ?]; reflexivity.
-  Qed.
-
-  Lemma toList_step_app :
-    forall prevs : list (bintree Elem),
-    forall nexts : list (bintree Elem),
-    toList_step (prevs ++ nexts) =
-    extract_elements prevs ++ toList_step (nexts ++ extract_children prevs).
-  Proof with eauto with *.
-    induction prevs as [ | [ | t_l t_e t_r] prevs IH]; simpl.
-    all: intros nexts; autorewrite with list...
-    { rewrite toList_step_unfold... }
-    { rewrite toList_step_unfold, <- app_assoc, IH, <- app_assoc... }
-  Qed.
-
-  Theorem toList_step_spec :
-    forall ts : list (bintree Elem),
-    toList_step ts =
-    extract_elements ts ++ toList_step (extract_children ts).
-  Proof.
-    intros ts. replace (ts) with (ts ++ []) at 1.
-    - exact (toList_step_app ts []).
-    - apply app_nil_r.
-  Qed.
-
-  Definition toList (root : bintree Elem) : list Elem :=
-    toList_step [root]
-  .
-
-  End BINARY_TREE_ACCESSORIES.
+  End BINARYTREE_BASIC_OPERATIONS.
+*)
 
 End BinaryTrees.
